hashedelgamal.ec
@@ -1,0 +1,113 @@
+(* Hashed el'gamal proof *)
+
+require import AllCore Distr.
+
+type group.
+
+op gid: group.
+
+op (^^): group -> group -> group.
+
+axiom grpA (x y z : group) : x ^^ y ^^ z = x ^^ (y ^^ z).
+
+axiom grpI (x  : group) : x ^^ gid = x.
+
+axiom grpC (x y : group) : x ^^ y = y ^^ x.
+
+  (* exponent definitions *)
+
+type exp.
+
+op (+*) : exp -> exp -> exp.
+
+axiom expA (x y z : exp) : x +* y +* z = x +* (y +* z).
+
+axiom expC (x y : exp) : x +* y = y +* x.
+
+op dexp : exp distr.
+
+op g : group.
+
+op (^) : group -> exp -> group.
+
+  (* forall (x : group), unique (q : exp), s.t. x = g^q *)
+
+axiom uni : forall (x : group), exists (q : exp),  x = g ^ q.
+
+axiom grexpA (q1 q2 : exp) : (g ^ q1) ^ q2 = g ^ (q1 +* q2).
+
+lemma grexpAll (x : group) (q1 q2 : exp) : (x ^ q1) ^q2 = x ^ (q1 +* q2).
+    proof.
+      admit.
+    
+  qed.
+
+      (* text definitions *)
+type text.
+
+op (+^) : text -> text -> text.
+
+axiom textA (x y z : text) : x +^ y +^ z = x +^ (y +^ z).
+
+op text0 : text.
+
+axiom textC (x y : text) : x +^ y = y +^ x.
+
+axiom textI (x : text) : x +^ text0 = x.
+
+axiom textR (x : text) : x +^ x = text0.
+
+op dtext : text distr.
+
+
+      (* Random Oracle *)
+module type RO = {
+  proc * init() : unit
+
+  proc f(x : group) : text
+}.
+
+module RO : RO = {
+  var mp : (group, text) fmap (* finite map, table *)
+
+     x1 -> t1
+     x2 -> t2
+     x3 -> t3
+
+  proc init() : unit = {
+    mp <- empty;  (* empty map *)
+  }
+
+  proc f(x : group) : text = {
+    var y : text;
+    if (x \notin mp) { (* not in mp's domain *)
+      y <$ dtext;   (* updating mp so as before but value of *)
+      mp.[x] <- y;  (* x is what we randomly picked *)
+    }
+    return oget mp.[x]; (* mp.[x] is either None or Some t *)
+  }
+}
+
+module HEG (RO : RO) ={
+  proc key_gen() : exp = {
+    var q : exp;
+    q <$ dexp;
+    return (g ^ q, q);
+  }
+
+  proc enc(e : exp, t : text) : group {
+    
+
+  }
+
+  proc dec(e : exp, g : group) : text {
+  }
+
+}
+
+
+  
+
+
+
+
